implement store with new approach and trying to prove some lemmas

BoogieLang/MapExample.thy
@@ -17,7 +17,7 @@ value "IntV 2 :: unit valn"
 definition simple_map_example :: "(unit val3, unit valn) map" where
   "simple_map_example = [Up ( Up (Up (IntV 1))) \<mapsto> IntV 2]"
 
-abbreviation MapTV where "MapTV \<equiv> MapV (TPrim TInt) (TPrim TInt)"  (* convenience for testing purposes *)
+abbreviation MapTV where "MapTV \<equiv> MapV [] (TPrim TInt)"  (* convenience for testing purposes *)
 abbreviation Up2 where "Up2 x \<equiv> Up (Up x)"
 abbreviation Up3 where "Up3 x \<equiv> Up (Up2 x)"
 abbreviation Up4 where "Up4 x \<equiv> Up (Up3 x)"
@@ -32,32 +32,37 @@ abbreviation m33 :: "unit val3" where "m33 \<equiv> MapAux [m22 \<mapsto> Up3 (I
 abbreviation m34 :: "unit valn" where "m34 \<equiv> MapTV  m33"
 
 abbreviation mg3 :: "unit val3" where "mg3 \<equiv> MapAux [m22 \<mapsto> Up2 m11]"
-abbreviation mg4 :: "unit valn" where "mg4 \<equiv> MapTV  mg3"
+abbreviation mg4 :: "unit valn" where "mg4 \<equiv> MapV [] (TMap []  (TPrim TInt)) mg3"
 
 (* there needs to be as many additional store functions, as there are nesting levels *)
 (* user needs to generate these functions (is there a way to make this cleaner, macro?) *)
-fun select3 :: "('a, _) val \<Rightarrow> ('a, _) val option \<rightharpoonup> ('a, _) val" where
-    "select3 (MapV tk tv (Inl f)) (Some k) = f k"
-  | "select3 _ _ = None"
-
-fun select2 :: "('a, _) val \<Rightarrow> ('a, _) val option \<rightharpoonup> ('a, _) val" where
-    "select2 (MapV tk tv (Inl f)) (Some k) = f k"
-  | "select2 (MapV tk tv (Inr m)) (Some k) = map_option up (select3 m (down k))"
-  | "select2 _ _ = None"
-
-fun select1 :: "('a, _) val \<Rightarrow> ('a, _) val option \<rightharpoonup> ('a, _) val" where
-    "select1 (MapV tk tv (Inl f)) (Some k) = f k"
-  | "select1 (MapV tk tv (Inr m)) (Some k) = map_option up (select2 m (down k))"
-  | "select1 _ _ = None"
-
-fun select0 :: "_ M \<Rightarrow> _ M option \<rightharpoonup> ('a, _) val" where
-    "select0 (MapAux m) (Some k) = m k"
-  (*| "select0 (MapV tk tv (Inr m)) (Some k) = map_option up (select1 m (down k))"*)
+fun select0 :: "_ M \<Rightarrow> _ M \<rightharpoonup> _ M" where
+    "select0 (MapAux m) (Up k) = m k"
   | "select0 _ _ = None"
 
+fun select1 :: "_ M \<Rightarrow> _ M \<rightharpoonup> _ M" where
+    "select1 (MapAux m) (Up k) = m k"
+  | "select1 (Up m) (Up k) = map_option Up (select0 m k)"
+  | "select1 _ _ = None"
+
+fun select2 :: "_ M \<Rightarrow> _ M \<rightharpoonup> _ M" where
+    "select2 (MapAux m) (Up k) = m k"
+  | "select2 (Up m) (Up k) = map_option Up (select1 m k)"
+  | "select2 _ _ = None"
+
+primrec valtoM :: "'a valn \<Rightarrow> _ M" where
+    "valtoM (MapV _ _ m) = m"
+  | "valtoM (LitV v) = Up3 (LitV v)"
+  | "valtoM (AbsV v) = Up3 (AbsV v)"
+
+fun MtoVal :: " _ M option \<Rightarrow> ty \<rightharpoonup> 'a valn" where
+    "MtoVal (Some (Up3 (LitV v))) _ = Some (LitV v)"
+  | "MtoVal (Some (Up3 (AbsV v))) _ = Some (AbsV v)"
+  | "MtoVal (Some x) (TMap tks tv) = Some (MapV tks tv x)"
+  | "MtoVal _ _ = None"
+
 primrec select_impl :: "'a valn \<Rightarrow> 'a valn \<rightharpoonup> 'a valn" where
-    "select_impl (MapV _ _ m) (MapV _ _ k) = select0 m (down k)"
-  | "select_impl (MapV _ _ m) (LitV v) = select0 m (Up3 (LitV v))"
+    "select_impl (MapV _ tv m) k = MtoVal (select2 m (valtoM k)) tv"
   | "select_impl (LitV _) _ = None"
   | "select_impl (AbsV _) _ = None"
 
@@ -67,28 +72,22 @@ abbreviation example_map :: "('a, 'a val3) map_interface" where
 
 lemma "(map_select example_map) mg4 m24 = Some m14" by simp
 
-
-fun store3 :: "('a, _) val \<Rightarrow> ('a, _) val option \<Rightarrow> ('a, _) val option \<rightharpoonup> ('a, _) val" where
-    "store3 (MapV tk tv (Inl f)) (Some k) (Some v) = Some (MapV tk tv (Inl (f(k \<mapsto> v))))"  
-  | "store3 _ _ _ = None"
-
-fun store2 :: "('a, _) val \<Rightarrow> ('a, _) val option \<Rightarrow> ('a, _) val option \<rightharpoonup> ('a, _) val" where
-    "store2 (MapV tk tv (Inl f)) (Some k) (Some v) = Some (MapV tk tv (Inl (f(k \<mapsto> v))))"
-  | "store2 (MapV tk tv (Inr m)) (Some k) (Some v) = map_option up (store3 m (down k) (down v))"
-  | "store2 _ _ _ = None"
-
-fun store1 :: "('a, _) val \<Rightarrow> ('a, _) val option \<Rightarrow> ('a, _) val option \<rightharpoonup> ('a, _) val" where
-    "store1 (MapV tk tv (Inl f)) (Some k) (Some v) = Some (MapV tk tv (Inl (f(k \<mapsto> v))))"
-  | "store1 (MapV tk tv (Inr m)) (Some k) (Some v) = map_option up (store2 m (down k) (down v))"
-  | "store1 _ _ _ = None"
-
-fun store0 :: "('a, _) val \<Rightarrow> ('a, _) val option \<Rightarrow> ('a, _) val option \<rightharpoonup> ('a, _) val" where
-    "store0 (MapV tk tv (Inl f)) (Some k) (Some v) = Some (MapV tk tv (Inl (f(k \<mapsto> v))))"
-  | "store0 (MapV tk tv (Inr m)) (Some k) (Some v) = map_option up (store1 m (down k) (down v))"
+fun store0 :: "_ M \<Rightarrow> _ M \<Rightarrow> _ M \<rightharpoonup> _ M" where
+    "store0 (MapAux m) (Up k) v = Some (MapAux (m(k \<mapsto> v)))"
   | "store0 _ _ _ = None"
 
-primrec store_impl :: "'a val4 \<Rightarrow> ('a, _) val \<Rightarrow> ('a, _) val \<rightharpoonup> ('a, _) val" where
-    "store_impl (MapV tk tv m) k v = store0 (MapV tk tv m) (down k) (Some v)"
+fun store1 :: "_ M \<Rightarrow> _ M \<Rightarrow> _ M \<rightharpoonup> _ M" where
+    "store1 (MapAux m) (Up k) v = Some (MapAux (m(k \<mapsto> v)))"
+  | "store1 (Up m) (Up k) (Up v) = map_option Up (store0 m k v)"
+  | "store1 _ _ _ = None"
+
+fun store2 :: "_ M \<Rightarrow> _ M \<Rightarrow> _ M \<rightharpoonup> _ M" where
+    "store2 (MapAux m) (Up k) v = Some (MapAux (m(k \<mapsto> v)))"
+  | "store2 (Up m) (Up k) (Up v) = map_option Up (store1 m k v)"
+  | "store2 _ _ _ = None"
+
+primrec store_impl :: "'a valn \<Rightarrow> 'a valn \<Rightarrow> 'a valn \<rightharpoonup> 'a valn" where
+    "store_impl (MapV tks tv m) k v = MtoVal (store2 m (valtoM k) (valtoM v)) (TMap tks tv)"
   | "store_impl (LitV _) _ _ = None"
   | "store_impl (AbsV _) _ _ = None"
 
@@ -99,10 +98,80 @@ abbreviation example_map2 :: "('a, 'a val3) map_interface" where
 primrec select_option where "select_option (Some v) k = (map_select example_map2) v k"
 lemma "select_option ((map_store example_map2) mg4 m24 (IntV 42)) m24 = Some (IntV 42)" by simp
 
+fun Eq where "Eq (Some (MapV _ _ a)) (Some (MapV _ _ b)) = (a = b)" | "Eq a b = (a = b)"
+
+fun wf :: "'a valn \<Rightarrow> bool" where
+    "wf (MapV _ _ (Up (Up (Up v)))) = False"
+  | "wf _ = True"
+
+
+
 lemma
-  assumes "(map_store example_map2) (MapV tk tv m) x v = Some ms"
-  shows "(map_select example_map2) ms x = Some v"
+  assumes store: "store_impl (MapV tks tv m) x v = Some ms"
+  assumes wf: "wf v"
+  assumes select: "select_impl ms x = Some w"
+  shows sh: "Eq (Some w) (Some v)"
+  oops
+
+
+lemma update0:
+  assumes "store0 m k v = Some ms"
+  assumes "select0 ms k = Some w"
+  shows "w = v"  
+  using assms(1,2) store0.elims by force
+
+
+lemma update1Up:
+  fixes ms :: "'a M M"
+  assumes "store1 (Up m') k v = Some ms"
+  assumes s: "Some w = select1 ms k"
+  shows "w = v"
+  by (smt (verit) M.distinct(1) M.inject(2) assms(1) map_option_eq_Some
+      option.discI s select1.elims store1.elims update0)
+
+(*
+  by (smt (verit) M.distinct(1) M.inject(2) assms(1) map_option_eq_Some
+      option.discI s select1.elims store1.elims update0)
+*)
+
+(*
+lemma update1Map:
+  fixes ms :: "'a M M"
+  assumes "store1 (MapAux m') k v = Some ms"
+  assumes s: "Some w = select1 ms k"
+  shows "w = v"
+  by (smt (verit) M.distinct(1) assms(1) map_upd_Some_unfold option.discI s
+      select1.simps(1) store1.elims)
+
+lemma update1:
+  fixes ms :: "'a M M"
+  assumes "store1 m k v = Some ms"
+  assumes s: "Some w = select1 ms k"
+  shows "w = v"
+  by (smt (verit) M.distinct(1) assms(1) map_upd_Some_unfold option.discI s
+      select1.simps(1) store1.elims)
+
+lemma update2:
+  fixes ms :: "'a M M M"
+  assumes "store2 (Up m) k v = Some ms"
+  assumes s: "Some w = select1 ms k"
+  shows "w = v"
+
+
+proof -
   apply auto
-  try
+
+
+(*
+lemma
+  assumes store: "store_impl (MapV tks tv m) x v = Some ms"
+  assumes wf: "wf v"
+  assumes select: "select_impl ms x = Some w"
+  shows sh: "Eq (Some w) (Some v)"
+proof -
+  have "Some ms = MtoVal (store2 m (valtoM x) (valtoM v)) (TMap tks tv)" using store by auto
+*)
+
+*)
 
 end
